<?xml version="1.0"?>
<rdf:RDF xmlns="http://www.ease-crc.org/ont/SOMA.owl#"
     xml:base="http://www.ease-crc.org/ont/SOMA.owl"
     xmlns:owl="http://www.w3.org/2002/07/owl#"
     xmlns:rdf="http://www.w3.org/1999/02/22-rdf-syntax-ns#"
     xmlns:xml="http://www.w3.org/XML/1998/namespace"
     xmlns:xsd="http://www.w3.org/2001/XMLSchema#"
     xmlns:SOMA="http://www.ease-crc.org/ont/SOMA.owl#"
     xmlns:rdfs="http://www.w3.org/2000/01/rdf-schema#">
    <owl:Ontology rdf:about="http://www.ease-crc.org/ont/SOMA.owl">
        <owl:imports rdf:resource="http://www.ontologydesignpatterns.org/ont/dul/DUL.owl"/>
    </owl:Ontology>
    


    <!-- 
    ///////////////////////////////////////////////////////////////////////////////////////
    //
    // Object Properties
    //
    ///////////////////////////////////////////////////////////////////////////////////////
     -->

    


    <!-- http://www.ease-crc.org/ont/SOMA.owl#hasInitialScene -->

    <owl:ObjectProperty rdf:about="http://www.ease-crc.org/ont/SOMA.owl#hasInitialScene">
        <rdfs:subPropertyOf rdf:resource="http://www.ontologydesignpatterns.org/ont/dul/DUL.owl#includesObject"/>
        <rdf:type rdf:resource="http://www.w3.org/2002/07/owl#AsymmetricProperty"/>
        <rdf:type rdf:resource="http://www.w3.org/2002/07/owl#IrreflexiveProperty"/>
        <rdfs:domain rdf:resource="http://www.ease-crc.org/ont/SOMA.owl#StateTransition"/>
        <rdfs:range rdf:resource="http://www.ease-crc.org/ont/SOMA.owl#Scene"/>
        <rdfs:comment>A relation between StateTransitions and Scenes, which identifies the scene the transition starts from.</rdfs:comment>
    </owl:ObjectProperty>
    


    <!-- http://www.ease-crc.org/ont/SOMA.owl#hasTerminalScene -->

    <owl:ObjectProperty rdf:about="http://www.ease-crc.org/ont/SOMA.owl#hasTerminalScene">
        <rdfs:subPropertyOf rdf:resource="http://www.ontologydesignpatterns.org/ont/dul/DUL.owl#includesObject"/>
        <rdf:type rdf:resource="http://www.w3.org/2002/07/owl#AsymmetricProperty"/>
        <rdf:type rdf:resource="http://www.w3.org/2002/07/owl#IrreflexiveProperty"/>
        <rdfs:domain rdf:resource="http://www.ease-crc.org/ont/SOMA.owl#StateTransition"/>
        <rdfs:range rdf:resource="http://www.ease-crc.org/ont/SOMA.owl#Scene"/>
        <rdfs:comment>A relation between StateTransitions and Scenes, which identifies the scene the transition is expected to end at.</rdfs:comment>
    </owl:ObjectProperty>
    


    <!-- 
    ///////////////////////////////////////////////////////////////////////////////////////
    //
    // Classes
    //
    ///////////////////////////////////////////////////////////////////////////////////////
     -->

    


    <!-- http://www.ease-crc.org/ont/SOMA.owl#Assertion -->

    <owl:Class rdf:about="http://www.ease-crc.org/ont/SOMA.owl#Assertion">
        <rdfs:subClassOf rdf:resource="http://www.ease-crc.org/ont/SOMA.owl#Illocution"/>
        <rdfs:subClassOf>
            <owl:Restriction>
                <owl:onProperty rdf:resource="http://www.ontologydesignpatterns.org/ont/dul/DUL.owl#classifies"/>
                <owl:allValuesFrom>
                    <owl:Restriction>
                        <owl:onProperty rdf:resource="http://www.ontologydesignpatterns.org/ont/dul/DUL.owl#hasParticipant"/>
                        <owl:someValuesFrom rdf:resource="http://www.ease-crc.org/ont/SOMA.owl#DeclarativeClause"/>
                    </owl:Restriction>
                </owl:allValuesFrom>
            </owl:Restriction>
        </rdfs:subClassOf>
    </owl:Class>
    


    <!-- http://www.ease-crc.org/ont/SOMA.owl#ClausalObject -->

    <owl:Class rdf:about="http://www.ease-crc.org/ont/SOMA.owl#ClausalObject">
        <rdfs:subClassOf rdf:resource="http://www.ease-crc.org/ont/SOMA.owl#LinguisticObject"/>
        <owl:disjointWith rdf:resource="http://www.ease-crc.org/ont/SOMA.owl#LexicalObject"/>
        <owl:disjointWith rdf:resource="http://www.ease-crc.org/ont/SOMA.owl#PhrasalObject"/>
        <rdfs:comment>A linguistic object that contains information which would be linguistically expressed as a clause.</rdfs:comment>
        <rdfs:label>Clausal object</rdfs:label>
    </owl:Class>
    


    <!-- http://www.ease-crc.org/ont/SOMA.owl#Command -->

    <owl:Class rdf:about="http://www.ease-crc.org/ont/SOMA.owl#Command">
        <rdfs:subClassOf rdf:resource="http://www.ease-crc.org/ont/SOMA.owl#Illocution"/>
        <rdfs:subClassOf>
            <owl:Restriction>
                <owl:onProperty rdf:resource="http://www.ontologydesignpatterns.org/ont/dul/DUL.owl#classifies"/>
                <owl:allValuesFrom>
                    <owl:Restriction>
                        <owl:onProperty rdf:resource="http://www.ontologydesignpatterns.org/ont/dul/DUL.owl#hasParticipant"/>
                        <owl:someValuesFrom rdf:resource="http://www.ease-crc.org/ont/SOMA.owl#ImperativeClause"/>
                    </owl:Restriction>
                </owl:allValuesFrom>
            </owl:Restriction>
        </rdfs:subClassOf>
    </owl:Class>
    


    <!-- http://www.ease-crc.org/ont/SOMA.owl#DeclarativeClause -->

    <owl:Class rdf:about="http://www.ease-crc.org/ont/SOMA.owl#DeclarativeClause">
        <rdfs:subClassOf rdf:resource="http://www.ease-crc.org/ont/SOMA.owl#ClausalObject"/>
        <rdfs:comment>A clause which makes an assertion or declaration.</rdfs:comment>
        <rdfs:label>Declarative clause</rdfs:label>
    </owl:Class>
    


    <!-- http://www.ease-crc.org/ont/SOMA.owl#Illocution -->

    <owl:Class rdf:about="http://www.ease-crc.org/ont/SOMA.owl#Illocution">
        <rdfs:subClassOf rdf:resource="http://www.ease-crc.org/ont/SOMA.owl#CommunicationTask"/>
        <rdfs:subClassOf>
            <owl:Restriction>
                <owl:onProperty rdf:resource="http://www.ontologydesignpatterns.org/ont/dul/DUL.owl#classifies"/>
                <owl:allValuesFrom rdf:resource="http://www.ease-crc.org/ont/SOMA.owl#Locution"/>
            </owl:Restriction>
        </rdfs:subClassOf>
        <rdfs:comment>A task which is executed by a Locution action.</rdfs:comment>
    </owl:Class>
    


    <!-- http://www.ease-crc.org/ont/SOMA.owl#ImageSchemaTheory -->

    <owl:Class rdf:about="http://www.ease-crc.org/ont/SOMA.owl#ImageSchemaTheory">
        <rdfs:subClassOf rdf:resource="http://www.ease-crc.org/ont/SOMA.owl#SchematicTheory"/>
        <rdfs:comment>A theory that describes an image-schematic relationship between some entities.

Image schemas are considered as fundamental, pre-conceptual, building blocks of cognition. They were introduced to characterize how human beings are believed to organize and make sense of experience.</rdfs:comment>
    </owl:Class>
    


    <!-- http://www.ease-crc.org/ont/SOMA.owl#ImperativeClause -->

    <owl:Class rdf:about="http://www.ease-crc.org/ont/SOMA.owl#ImperativeClause">
        <rdfs:subClassOf rdf:resource="http://www.ease-crc.org/ont/SOMA.owl#ClausalObject"/>
        <rdfs:subClassOf>
            <owl:Restriction>
                <owl:onProperty rdf:resource="http://www.ontologydesignpatterns.org/ont/dul/DUL.owl#expresses"/>
                <owl:someValuesFrom rdf:resource="http://www.ease-crc.org/ont/SOMA.owl#StateTransition"/>
            </owl:Restriction>
        </rdfs:subClassOf>
        <rdfs:subClassOf>
            <owl:Restriction>
                <owl:onProperty rdf:resource="http://www.ontologydesignpatterns.org/ont/dul/DUL.owl#expresses"/>
                <owl:allValuesFrom rdf:resource="http://www.ease-crc.org/ont/SOMA.owl#StateTransition"/>
            </owl:Restriction>
        </rdfs:subClassOf>
        <rdfs:comment>A clause which commands some agent to perform a task or bring about a state of affairs.</rdfs:comment>
        <rdfs:label>Imperative clause</rdfs:label>
    </owl:Class>
    


    <!-- http://www.ease-crc.org/ont/SOMA.owl#InterrogativeClause -->

    <owl:Class rdf:about="http://www.ease-crc.org/ont/SOMA.owl#InterrogativeClause">
        <rdfs:subClassOf rdf:resource="http://www.ease-crc.org/ont/SOMA.owl#ClausalObject"/>
        <rdfs:comment>A clause which makes a request, typically information, of some agent.

Note that in a semantic sense such clauses always request information, but in a pragmatic sense they can be used to convey commands or requests for action, such as e.g. &quot;can you close the door?&quot; The question is not just a request for information about ability, but a request to perform a task.</rdfs:comment>
        <rdfs:label>Interrogative clause</rdfs:label>
    </owl:Class>
    


    <!-- http://www.ease-crc.org/ont/SOMA.owl#LexicalObject -->

    <owl:Class rdf:about="http://www.ease-crc.org/ont/SOMA.owl#LexicalObject">
        <rdfs:subClassOf rdf:resource="http://www.ease-crc.org/ont/SOMA.owl#LinguisticObject"/>
        <owl:disjointWith rdf:resource="http://www.ease-crc.org/ont/SOMA.owl#PhrasalObject"/>
        <rdfs:comment>A linguistic object that contains information which would be linguistically expressed as a lexical item (loosely speaking, a word).</rdfs:comment>
        <rdfs:label>Lexical object</rdfs:label>
    </owl:Class>
    


    <!-- http://www.ease-crc.org/ont/SOMA.owl#LinguisticObject -->

    <owl:Class rdf:about="http://www.ease-crc.org/ont/SOMA.owl#LinguisticObject">
        <rdfs:subClassOf rdf:resource="http://www.ontologydesignpatterns.org/ont/dul/DUL.owl#InformationObject"/>
        <rdfs:comment>An information bearing object that is used to analyze some linguistic production.</rdfs:comment>
        <rdfs:label>Linguistic object</rdfs:label>
    </owl:Class>
    


    <!-- http://www.ease-crc.org/ont/SOMA.owl#Locution -->

    <owl:Class rdf:about="http://www.ease-crc.org/ont/SOMA.owl#Locution">
        <rdfs:subClassOf rdf:resource="http://www.ease-crc.org/ont/SOMA.owl#InterpretedAction"/>
        <rdfs:subClassOf>
            <owl:Restriction>
                <owl:onProperty rdf:resource="http://www.ontologydesignpatterns.org/ont/dul/DUL.owl#hasParticipant"/>
                <owl:someValuesFrom rdf:resource="http://www.ease-crc.org/ont/SOMA.owl#LinguisticObject"/>
            </owl:Restriction>
        </rdfs:subClassOf>
        <rdfs:comment>An action in which an agent uses some actuator for communication purposes.</rdfs:comment>
    </owl:Class>
    


    <!-- http://www.ease-crc.org/ont/SOMA.owl#PhrasalObject -->

    <owl:Class rdf:about="http://www.ease-crc.org/ont/SOMA.owl#PhrasalObject">
        <rdfs:subClassOf rdf:resource="http://www.ease-crc.org/ont/SOMA.owl#LinguisticObject"/>
        <rdfs:comment>A linguistic object that contains information which would be linguistically expressed as a phrase.</rdfs:comment>
        <rdfs:label>Phrasal object</rdfs:label>
    </owl:Class>
    


    <!-- http://www.ease-crc.org/ont/SOMA.owl#Query -->

    <owl:Class rdf:about="http://www.ease-crc.org/ont/SOMA.owl#Query">
        <rdfs:subClassOf rdf:resource="http://www.ease-crc.org/ont/SOMA.owl#Illocution"/>
        <rdfs:subClassOf>
            <owl:Restriction>
                <owl:onProperty rdf:resource="http://www.ontologydesignpatterns.org/ont/dul/DUL.owl#classifies"/>
                <owl:allValuesFrom>
                    <owl:Restriction>
                        <owl:onProperty rdf:resource="http://www.ontologydesignpatterns.org/ont/dul/DUL.owl#hasParticipant"/>
                        <owl:someValuesFrom rdf:resource="http://www.ease-crc.org/ont/SOMA.owl#InterrogativeClause"/>
                    </owl:Restriction>
                </owl:allValuesFrom>
            </owl:Restriction>
        </rdfs:subClassOf>
    </owl:Class>
    


    <!-- http://www.ease-crc.org/ont/SOMA.owl#Scene -->

    <owl:Class rdf:about="http://www.ease-crc.org/ont/SOMA.owl#Scene">
        <rdfs:subClassOf rdf:resource="http://www.ontologydesignpatterns.org/ont/dul/DUL.owl#Situation"/>
        <rdfs:subClassOf>
            <owl:Restriction>
                <owl:onProperty rdf:resource="http://www.ontologydesignpatterns.org/ont/dul/DUL.owl#includesEvent"/>
                <owl:someValuesFrom rdf:resource="http://www.ease-crc.org/ont/SOMA.owl#State"/>
            </owl:Restriction>
        </rdfs:subClassOf>
        <rdfs:subClassOf>
            <owl:Restriction>
                <owl:onProperty rdf:resource="http://www.ontologydesignpatterns.org/ont/dul/DUL.owl#satisfies"/>
                <owl:someValuesFrom rdf:resource="http://www.ease-crc.org/ont/SOMA.owl#ImageSchemaTheory"/>
            </owl:Restriction>
        </rdfs:subClassOf>
        <rdfs:comment>Scenes are Situations which interpret a State in terms of its conformance to some qualitative, image schematic description. I.e., the scene is described in terms of qualitative functional and spatial relations existing between participating objects.</rdfs:comment>
    </owl:Class>
    


    <!-- http://www.ease-crc.org/ont/SOMA.owl#SchematicTheory -->

    <owl:Class rdf:about="http://www.ease-crc.org/ont/SOMA.owl#SchematicTheory">
        <rdfs:subClassOf rdf:resource="http://www.ontologydesignpatterns.org/ont/dul/DUL.owl#Theory"/>
        <rdfs:comment>A theory used to describe, analyze, and reason with the meaning of a linguistic message.

Note that such theories are useful both when analyzing an actual linguistic production, and when creating a linguistic production to describe some observed experience.</rdfs:comment>
    </owl:Class>
    


    <!-- http://www.ease-crc.org/ont/SOMA.owl#StateTransition -->

    <owl:Class rdf:about="http://www.ease-crc.org/ont/SOMA.owl#StateTransition">
        <rdfs:subClassOf rdf:resource="http://www.ontologydesignpatterns.org/ont/dul/DUL.owl#Transition"/>
        <rdfs:subClassOf>
            <owl:Restriction>
                <owl:onProperty rdf:resource="http://www.ease-crc.org/ont/SOMA.owl#hasInitialScene"/>
                <owl:someValuesFrom rdf:resource="http://www.ease-crc.org/ont/SOMA.owl#Scene"/>
            </owl:Restriction>
        </rdfs:subClassOf>
        <rdfs:subClassOf>
            <owl:Restriction>
                <owl:onProperty rdf:resource="http://www.ease-crc.org/ont/SOMA.owl#hasTerminalScene"/>
                <owl:someValuesFrom rdf:resource="http://www.ease-crc.org/ont/SOMA.owl#Scene"/>
            </owl:Restriction>
        </rdfs:subClassOf>
        <rdfs:subClassOf>
            <owl:Restriction>
                <owl:onProperty rdf:resource="http://www.ontologydesignpatterns.org/ont/dul/DUL.owl#includesEvent"/>
                <owl:someValuesFrom rdf:resource="http://www.ontologydesignpatterns.org/ont/dul/DUL.owl#Action"/>
            </owl:Restriction>
        </rdfs:subClassOf>
        <rdfs:subClassOf>
            <owl:Restriction>
                <owl:onProperty rdf:resource="http://www.ontologydesignpatterns.org/ont/dul/DUL.owl#satisfies"/>
                <owl:someValuesFrom rdf:resource="http://www.ease-crc.org/ont/SOMA.owl#ImageSchemaTheory"/>
            </owl:Restriction>
        </rdfs:subClassOf>
        <rdfs:comment>A transition between two states brought about by the Action of some Agent.</rdfs:comment>
    </owl:Class>
</rdf:RDF>



<!-- Generated by the OWL API (version 4.5.9.2019-02-01T07:24:44Z) https://github.com/owlcs/owlapi -->

