<?xml version="1.0"?>
<rdf:RDF xmlns="http://www.ease-crc.org/ont/SOMA-TSD.owl#"
     xml:base="http://www.ease-crc.org/ont/SOMA-TSD.owl"
     xmlns:dc="http://purl.org/dc/elements/1.1/"
     xmlns:owl="http://www.w3.org/2002/07/owl#"
     xmlns:rdf="http://www.w3.org/1999/02/22-rdf-syntax-ns#"
     xmlns:xml="http://www.w3.org/XML/1998/namespace"
     xmlns:xsd="http://www.w3.org/2001/XMLSchema#"
     xmlns:SOMA="http://www.ease-crc.org/ont/SOMA.owl#"
     xmlns:rdfs="http://www.w3.org/2000/01/rdf-schema#">
    <owl:Ontology rdf:about="http://www.ease-crc.org/ont/SOMA-TSD.owl">
        <owl:imports rdf:resource="http://www.ease-crc.org/ont/SOMA-ACT.owl"/>
        <owl:imports rdf:resource="http://www.ease-crc.org/ont/SOMA-HOME.owl"/>
        <owl:imports rdf:resource="http://www.ease-crc.org/ont/SOMA-OBJ.owl"/>
        <owl:imports rdf:resource="http://www.ease-crc.org/ont/SOMA.owl"/>
        <owl:imports rdf:resource="http://www.ontologydesignpatterns.org/ont/dul/DUL.owl"/>
    </owl:Ontology>
    


    <!-- 
    ///////////////////////////////////////////////////////////////////////////////////////
    //
    // Classes
    //
    ///////////////////////////////////////////////////////////////////////////////////////
     -->

    


    <!-- http://www.ease-crc.org/ont/SOMA.owl#Spoon -->

    <owl:Class rdf:about="http://www.ease-crc.org/ont/SOMA.owl#Spoon">
        <rdfs:subClassOf rdf:resource="http://www.ease-crc.org/ont/SOMA.owl#Cutlery"/>
    </owl:Class>
    


    <!-- http://www.ease-crc.org/ont/SOMA.owl#TableSpoon -->

    <owl:Class rdf:about="http://www.ease-crc.org/ont/SOMA.owl#TableSpoon">
        <rdfs:subClassOf rdf:resource="http://www.ease-crc.org/ont/SOMA.owl#Spoon"/>
    </owl:Class>
    


    <!-- http://www.ease-crc.org/ont/SOMA.owl#TeaSpoon -->

    <owl:Class rdf:about="http://www.ease-crc.org/ont/SOMA.owl#TeaSpoon">
        <rdfs:subClassOf rdf:resource="http://www.ease-crc.org/ont/SOMA.owl#Spoon"/>
    </owl:Class>
    


    <!-- http://www.ease-crc.org/ont/SOMA.owl#Box -->

    <owl:Class rdf:about="http://www.ease-crc.org/ont/SOMA.owl#Box">
        <rdfs:subClassOf rdf:resource="http://www.ease-crc.org/ont/SOMA.owl#DesignedContainer"/>
        <rdfs:comment>A cuboid-shaped container.</rdfs:comment>
    </owl:Class>
    


    <!-- http://www.ease-crc.org/ont/SOMA.owl#BreadKnife -->

    <owl:Class rdf:about="http://www.ease-crc.org/ont/SOMA.owl#BreadKnife">
        <rdfs:subClassOf rdf:resource="http://www.ease-crc.org/ont/SOMA.owl#Knife"/>
        <rdfs:comment>Knife to cut break.</rdfs:comment>
    </owl:Class>
    


    <!-- http://www.ease-crc.org/ont/SOMA.owl#Carafe -->

    <owl:Class rdf:about="http://www.ease-crc.org/ont/SOMA.owl#Carafe">
        <rdfs:subClassOf rdf:resource="http://www.ease-crc.org/ont/SOMA.owl#DesignedContainer"/>
        <rdfs:comment>A container used to hold and pour some beverage.</rdfs:comment>
    </owl:Class>
    


    <!-- http://www.ease-crc.org/ont/SOMA.owl#CerealBox -->

    <owl:Class rdf:about="http://www.ease-crc.org/ont/SOMA.owl#CerealBox">
        <rdfs:subClassOf rdf:resource="http://www.ease-crc.org/ont/SOMA.owl#Box"/>
        <rdfs:comment>A box which holds, or at least is intended to usually hold, cereal flakes.</rdfs:comment>
    </owl:Class>
    


    <!-- http://www.ease-crc.org/ont/SOMA.owl#CoffeeCarafe -->

    <owl:Class rdf:about="http://www.ease-crc.org/ont/SOMA.owl#CoffeeCarafe">
        <rdfs:subClassOf rdf:resource="http://www.ease-crc.org/ont/SOMA.owl#Carafe"/>
        <rdfs:comment>A carafe which holds, or at least is intended to usually hold, coffee.</rdfs:comment>
    </owl:Class>
    


    <!-- http://www.ease-crc.org/ont/SOMA.owl#DessertFork -->

    <owl:Class rdf:about="http://www.ease-crc.org/ont/SOMA.owl#DessertFork">
        <rdfs:subClassOf rdf:resource="http://www.ease-crc.org/ont/SOMA.owl#Fork"/>
        <rdfs:comment>Small fork for eating dessert like cake.</rdfs:comment>
    </owl:Class>
    


    <!-- http://www.ease-crc.org/ont/SOMA.owl#DinnerPlate -->

    <owl:Class rdf:about="http://www.ease-crc.org/ont/SOMA.owl#DinnerPlate">
        <rdfs:subClassOf rdf:resource="http://www.ease-crc.org/ont/SOMA.owl#Plate"/>
        <rdfs:comment>Regular size plate for eating a main dish.</rdfs:comment>
    </owl:Class>
    


    <!-- http://www.ease-crc.org/ont/SOMA.owl#Dispenser -->

    <owl:Class rdf:about="http://www.ease-crc.org/ont/SOMA.owl#Dispenser">
        <rdfs:subClassOf rdf:resource="http://www.ease-crc.org/ont/SOMA.owl#DesignedContainer"/>
        <rdfs:comment>A small container used to store and serve some flavoring substance for a dish or beverage.</rdfs:comment>
    </owl:Class>
    


    <!-- http://www.ease-crc.org/ont/SOMA.owl#Glass -->

    <owl:Class rdf:about="http://www.ease-crc.org/ont/SOMA.owl#Glass">
        <rdfs:subClassOf rdf:resource="http://www.ease-crc.org/ont/SOMA.owl#Crockery"/>
        <rdfs:comment>A container made usually from glass or transparent plastic which is used to hold, typically cold, beverages.</rdfs:comment>
    </owl:Class>
    


    <!-- http://www.ease-crc.org/ont/SOMA.owl#JamJar -->

    <owl:Class rdf:about="http://www.ease-crc.org/ont/SOMA.owl#JamJar">
        <rdfs:subClassOf rdf:resource="http://www.ease-crc.org/ont/SOMA.owl#Jar"/>
        <rdfs:comment>A jar which holds, or at least is intended to usually hold, jam.</rdfs:comment>
    </owl:Class>
    


    <!-- http://www.ease-crc.org/ont/SOMA.owl#Jar -->

    <owl:Class rdf:about="http://www.ease-crc.org/ont/SOMA.owl#Jar">
        <rdfs:subClassOf rdf:resource="http://www.ease-crc.org/ont/SOMA.owl#DesignedContainer"/>
        <rdfs:comment>A container used for long-term storage of some liquid or viscous dish.</rdfs:comment>
    </owl:Class>
    


    <!-- http://www.ease-crc.org/ont/SOMA.owl#MilkBottle -->

    <owl:Class rdf:about="http://www.ease-crc.org/ont/SOMA.owl#MilkBottle">
        <rdfs:subClassOf rdf:resource="http://www.ease-crc.org/ont/SOMA.owl#Bottle"/>
        <rdfs:comment>A bottle which holds, or at least is intended to usually hold, milk.</rdfs:comment>
    </owl:Class>
    


    <!-- http://www.ease-crc.org/ont/SOMA.owl#MilkPack -->

    <owl:Class rdf:about="http://www.ease-crc.org/ont/SOMA.owl#MilkPack">
        <rdfs:subClassOf rdf:resource="http://www.ease-crc.org/ont/SOMA.owl#Pack"/>
        <rdfs:comment>A pack which holds, or at least is intended to usually hold, milk.</rdfs:comment>
    </owl:Class>
    


    <!-- http://www.ease-crc.org/ont/SOMA.owl#NutellaJar -->

    <owl:Class rdf:about="http://www.ease-crc.org/ont/SOMA.owl#NutellaJar">
        <rdfs:subClassOf rdf:resource="http://www.ease-crc.org/ont/SOMA.owl#Jar"/>
        <rdfs:comment>A jar which holds, or at least is intended to usually hold, Nutella.</rdfs:comment>
    </owl:Class>
    


    <!-- http://www.ease-crc.org/ont/SOMA.owl#PastaBowl -->

    <owl:Class rdf:about="http://www.ease-crc.org/ont/SOMA.owl#PastaBowl">
        <rdfs:subClassOf rdf:resource="http://www.ease-crc.org/ont/SOMA.owl#Bowl"/>
        <rdfs:comment>A bowl which holds, or at least is intended to usually hold, pasta.</rdfs:comment>
    </owl:Class>
    


    <!-- http://www.ease-crc.org/ont/SOMA.owl#PepperShaker -->

    <owl:Class rdf:about="http://www.ease-crc.org/ont/SOMA.owl#PepperShaker">
        <rdfs:subClassOf rdf:resource="http://www.ease-crc.org/ont/SOMA.owl#Shaker"/>
        <rdfs:comment>A shaker which holds, or at least is intended to usually hold, pepper.</rdfs:comment>
    </owl:Class>
    


    <!-- http://www.ease-crc.org/ont/SOMA.owl#RaspberryJamJar -->

    <owl:Class rdf:about="http://www.ease-crc.org/ont/SOMA.owl#RaspberryJamJar">
        <rdfs:subClassOf rdf:resource="http://www.ease-crc.org/ont/SOMA.owl#JamJar"/>
        <rdfs:comment>A jar which holds, or at least is intended to usually hold, raspberry jam.</rdfs:comment>
    </owl:Class>
    


    <!-- http://www.ease-crc.org/ont/SOMA.owl#SaladBowl -->

    <owl:Class rdf:about="http://www.ease-crc.org/ont/SOMA.owl#SaladBowl">
        <rdfs:subClassOf rdf:resource="http://www.ease-crc.org/ont/SOMA.owl#Bowl"/>
        <rdfs:comment>A bowl which holds, or at least is intended to usually hold, salad.</rdfs:comment>
    </owl:Class>
    


    <!-- http://www.ease-crc.org/ont/SOMA.owl#SaltShaker -->

    <owl:Class rdf:about="http://www.ease-crc.org/ont/SOMA.owl#SaltShaker">
        <rdfs:subClassOf rdf:resource="http://www.ease-crc.org/ont/SOMA.owl#Shaker"/>
        <rdfs:comment>A shaker which holds, or at least is intended to usually hold, salt.</rdfs:comment>
    </owl:Class>
    


    <!-- http://www.ease-crc.org/ont/SOMA.owl#Shaker -->

    <owl:Class rdf:about="http://www.ease-crc.org/ont/SOMA.owl#Shaker">
        <rdfs:subClassOf rdf:resource="http://www.ease-crc.org/ont/SOMA.owl#DesignedContainer"/>
    </owl:Class>
    


    <!-- http://www.ease-crc.org/ont/SOMA.owl#SidePlate -->

    <owl:Class rdf:about="http://www.ease-crc.org/ont/SOMA.owl#SidePlate">
        <rdfs:subClassOf rdf:resource="http://www.ease-crc.org/ont/SOMA.owl#Plate"/>
        <rdfs:comment>Small plate e.g. used for bread in breakfast or dinner.</rdfs:comment>
    </owl:Class>
    


    <!-- http://www.ease-crc.org/ont/SOMA.owl#SoupPot -->

    <owl:Class rdf:about="http://www.ease-crc.org/ont/SOMA.owl#SoupPot">
        <rdfs:subClassOf rdf:resource="http://www.ease-crc.org/ont/SOMA.owl#Pot"/>
        <rdfs:comment>A pot which holds, or at least is intended to usually hold, soup.</rdfs:comment>
    </owl:Class>
    


    <!-- http://www.ease-crc.org/ont/SOMA.owl#SugarDispenser -->

    <owl:Class rdf:about="http://www.ease-crc.org/ont/SOMA.owl#SugarDispenser">
        <rdfs:subClassOf rdf:resource="http://www.ease-crc.org/ont/SOMA.owl#Dispenser"/>
    </owl:Class>
    


    <!-- http://www.ease-crc.org/ont/SOMA.owl#TableFork -->

    <owl:Class rdf:about="http://www.ease-crc.org/ont/SOMA.owl#TableFork">
        <rdfs:subClassOf rdf:resource="http://www.ease-crc.org/ont/SOMA.owl#Fork"/>
        <rdfs:comment>Regular eating fork, e.g. for Spaghetti.</rdfs:comment>
    </owl:Class>
    


    <!-- http://www.ease-crc.org/ont/SOMA.owl#TableKnife -->

    <owl:Class rdf:about="http://www.ease-crc.org/ont/SOMA.owl#TableKnife">
        <rdfs:subClassOf rdf:resource="http://www.ease-crc.org/ont/SOMA.owl#Knife"/>
        <rdfs:comment>Regular knife used for eating or speading butter on bread.</rdfs:comment>
    </owl:Class>
    


    <!-- http://www.ease-crc.org/ont/SOMA.owl#WaterBottle -->

    <owl:Class rdf:about="http://www.ease-crc.org/ont/SOMA.owl#WaterBottle">
        <rdfs:subClassOf rdf:resource="http://www.ease-crc.org/ont/SOMA.owl#Bottle"/>
        <rdfs:comment>A bottle which holds, or at least is intended to usually hold, water.</rdfs:comment>
    </owl:Class>
    


    <!-- http://www.ease-crc.org/ont/SOMA.owl#WaterGlass -->

    <owl:Class rdf:about="http://www.ease-crc.org/ont/SOMA.owl#WaterGlass">
        <rdfs:subClassOf rdf:resource="http://www.ease-crc.org/ont/SOMA.owl#Glass"/>
        <rdfs:comment>A glass which holds, or at least is intended to usually hold, water.</rdfs:comment>
    </owl:Class>
    


    <!-- http://www.ease-crc.org/ont/SOMA.owl#WineBottle -->

    <owl:Class rdf:about="http://www.ease-crc.org/ont/SOMA.owl#WineBottle">
        <rdfs:subClassOf rdf:resource="http://www.ease-crc.org/ont/SOMA.owl#Bottle"/>
        <rdfs:comment>A bottle which holds, or at least is intended to usually hold, wine.</rdfs:comment>
    </owl:Class>
    


    <!-- http://www.ease-crc.org/ont/SOMA.owl#WineGlass -->

    <owl:Class rdf:about="http://www.ease-crc.org/ont/SOMA.owl#WineGlass">
        <rdfs:subClassOf rdf:resource="http://www.ease-crc.org/ont/SOMA.owl#Glass"/>
        <rdfs:comment>A glass which holds, or at least is intended to usually hold, wine.</rdfs:comment>
    </owl:Class>
</rdf:RDF>



<!-- Generated by the OWL API (version 4.5.9.2019-02-01T07:24:44Z) https://github.com/owlcs/owlapi -->

